Work on AVL trees

examples/avl.v
@@ -1,26 +1,26 @@
-Require Import Arith ZArith.
+Require Import Arith ZArith Compare_dec.
 
 Section Tree.
-  Inductive tree (X: Type) : Type :=
-    | Leaf: tree X
-    | Node: X -> tree X -> tree X -> tree X.
+  Inductive tree (A: Type) : Type :=
+    | Leaf: tree A
+    | Node: A -> tree A -> tree A -> tree A.
 
-  Implicit Arguments Leaf [[X]].
-  Implicit Arguments Node [[X]].
+  Implicit Arguments Leaf [[A]].
+  Implicit Arguments Node [[A]].
 
-  Fixpoint node_count {X: Type} (t: tree X) : nat :=
+  Fixpoint node_count {A: Type} (t: tree A) : nat :=
     match t with
     | Leaf       => 0
     | Node _ a b => 1 + node_count a + node_count b
     end.
 
-  Fixpoint tree_height {X: Type} (t: tree X) : nat :=
+  Fixpoint tree_height {A: Type} (t: tree A) : nat :=
     match t with
     | Leaf       => 0
     | Node _ a b => 1 + max (tree_height a) (tree_height b)
   end.
 
-  Theorem tree_height_le_count: forall X: Type, forall t: tree X,
+  Theorem tree_height_le_count: forall {A: Type}, forall t: tree A,
     tree_height t <= node_count t.
   Proof.
     intros X t. induction t as [| x a IHa b].
@@ -32,49 +32,68 @@ Section Tree.
         intro H. rewrite IHb. apply le_plus_r.
   Qed.
 
-  Fixpoint search {X: Type} (x: X) (t: tree X) : option X :=
-    match t with
-    | Leaf       => None
-    | Node y a b => match comp x y with
-      | LT => search x a
-      | EQ => Some y
-      | GT => search x b
-    end
-  end.
+  Section Search.
+    Inductive
 
-  Fixpoint insert (x: X) (t: tree X) : tree X :=
-    match t with
-    | Leaf       => Node x Leaf Leaf
-    | Node y a b => match comp x y with
-      | LT => Node y (insert x a) b
-      | EQ => Node x a b
-      | GT => Node y a (insert x b)
-    end
-  end.
+    Fixpoint search (x: nat) (t: tree nat) : option nat :=
+      match t with
+      | Leaf       => None
+      | Node y a b => match nat_compare x y with
+        | Lt => search x a
+        | Eq => Some y
+        | Gt => search x b
+      end
+    end.
 
-  Theorem insert_search: forall (x: X), forall (t: tree X),
-    search x (insert x t) = Some x.
-  Proof.
-    intros x t. induction t as [| y a IHa b].
-      simpl. admit.
+    Fixpoint insert (x: nat) (t: tree nat) : tree nat :=
+      match t with
+      | Leaf       => Node x Leaf Leaf
+      | Node y a b => match nat_compare x y with
+        | Lt => Node y (insert x a) b
+        | Eq => Node x a b
+        | Gt => Node y a (insert x b)
+      end
+    end.
+
+    Lemma nat_compare_refl: forall n: nat,
+      nat_compare n n = Eq.
+    Proof.
+      intros n. induction n as [| n'].
+        reflexivity.
+        simpl. apply IHn'.
+    Qed.
+
+    Theorem insert_search: forall (x: nat), forall (t: tree nat),
+      search x (insert x t) = Some x.
+    Proof.
+      intros x t. induction t as [| y a IHa b IHb].
+        (* t = Leaf *)
+        simpl. rewrite -> nat_compare_refl. reflexivity.
+        (* t = Node y a b *)
+        simpl. remember (nat_compare x y) as eq. destruct eq.
+          (* Eq *) simpl. rewrite nat_compare_refl. reflexivity.
+          (* Lt *) simpl. rewrite <- Heqeq. rewrite IHa. reflexivity.
+          (* Gt *) simpl. rewrite <- Heqeq. rewrite IHb. reflexivity.
+    Qed.
+  End Search.
 
   Section AVL.
     Open Scope Z_scope.
 
-    Definition balance_factor {X: Type} (t: tree X) : Z :=
+    Definition balance_factor (t: tree A) : Z :=
       match t with
       | Leaf       => 0
       | Node a _ b => Z.of_nat (tree_height a) - Z.of_nat (tree_height b)
       end.
 
-    Definition is_balanced {X: Type} (t: tree X) : Prop :=
+    Definition is_balanced (t: tree A) : Prop :=
       -1 <= balance_factor t <= 1.
 
-    Inductive AVL {X: Type} : tree X -> Prop :=
+    Inductive AVL : tree A -> Prop :=
       | avl_nil: AVL Leaf
       | avl_node: forall n, is_balanced n -> AVL n.
 
-    Fixpoint avl_insert {X: Type} (x: X) (t: tree X) : tree X :=
+    Fixpoint avl_insert (x: A) (t: tree A) : tree A :=
       match
   End AVL.
 End Tree.
